Invented a law for MonadReader. Added a class MonadFail. Defined instances of this class for list and option. Proved that RWS is MonadState and that Reader is MonadReader. Moved most functions from MonadPlus to MonadFail. Proved that lift preserves >> and used this to prove that transforming a MonadReader gives a MonadReader.

Instances/ListInst.v
@@ -188,3 +188,13 @@ Proof.
   intros. ext l.
   induction l as [| h t]; unfold compose in *; cbn; congruence.
 Defined.
+
+Require Import MonadClass.All.
+
+Definition fail_List {A : Type} : list A := [].
+
+Instance MonadFail_List : MonadFail list Monad_List :=
+{
+    fail := @fail_List
+}.
+Proof. intros. compute. reflexivity. Defined.
