MonadClass/MonadReader.v
@@ -1,11 +1,13 @@
 Require Import HSLib.Base.
 Require Import Control.Monad.
+Require Import Control.MonadTrans.
 
 Class MonadReader
   (R : Type) (M : Type -> Type) (inst : Monad M) : Type :=
 {
     ask : M R;
-    local : (R -> R) -> M R -> M R;
+(*    local : (R -> R) -> M R -> M R;*)
+    ask_ask : ask >> ask = ask;
 }.
 
 Section MonadReader_funs.
@@ -24,4 +26,14 @@ Definition asks {A : Type} (f : R -> A) : M A :=
 
 End MonadReader_funs.
 
-Check asks.
+Instance MonadReader_MonadTrans
+  (T : (Type -> Type) -> Type -> Type) (instT : MonadTrans T)
+  (M : Type -> Type) (instM : Monad M)
+  (R : Type) (instMR : MonadReader R M instM)
+  : MonadReader R (T M) (is_monad _ instM) :=
+{
+    ask := lift ask
+}.
+Proof.
+  rewrite lift_constrA, ask_ask. reflexivity.
+Defined.
