Control/MonadTrans.v
@@ -34,3 +34,16 @@ match goal with
           let x := fresh "x" in ext x;
           rewrite <- fmap_comp'; f_equal
 end.
+
+Lemma lift_constrA :
+  forall
+    (T : (Type -> Type) -> Type -> Type) (instT : MonadTrans T)
+    (M : Type -> Type) (instM : Monad M)
+    (A : Type) (x : M A),
+      @constrA (T M) (is_monad _ instM) _ _ (lift x) (lift x) =
+      @lift T instT M instM A (x >> x).
+Proof.
+  intros.
+    rewrite !constrA_spec.
+    rewrite lift_bind. unfold compose. reflexivity.
+Defined.
