MonadClass/All.v
@@ -1,0 +1,5 @@
+Require Export MonadClass.MonadSkip.
+Require Export MonadClass.MonadFail.
+Require Export MonadClass.MonadReader.
+Require Export MonadClass.MonadState.
+Require Export MonadClass.MonadFree.
