MonadClass/MonadFail.v
@@ -1,0 +1,72 @@
+Require Import HSLib.Base.
+Require Import Control.Monad.
+Require Import Control.Alternative.
+Require Import Control.Foldable.
+
+Class MonadFail (M : Type -> Type) (inst : Monad M) : Type :=
+{
+    fail : forall {A :  Type}, M A;
+    bind_fail_l :
+      forall (A B : Type) (f : A -> M B),
+        fail >>= f = fail
+}.
+
+Set Implicit Arguments.
+
+Section MonadFailFuns.
+
+Variables M : Type -> Type.
+Variable instM : Monad M.
+Variable instMF : MonadFail M instM.
+
+Definition mfilter {A : Type} (f : A -> bool) (ma : M A) : M A :=
+  ma >>= fun a : A => if f a then pure a else fail.
+
+Definition mpartition {A : Type} (p : A -> bool) (ma : M A) : M A * M A :=
+  (mfilter p ma, mfilter (p .> negb) ma).
+
+Definition fromOption {A : Type} (oa : option A) : M A :=
+match oa with
+    | None => fail
+    | Some a => pure a
+end.
+
+Definition mcatOptions {A : Type} (x : M (option A)) : M A :=
+  x >>= fromOption.
+Print afold.
+
+(** TODO: threw away mscatter and mconcatMap *)
+
+Definition sum_left {A B : Type} (x : A + B) : option A :=
+match x with
+    | inl a => Some a
+    | _ => None
+end.
+
+Definition sum_right {A B : Type} (x : A + B) : option B :=
+match x with
+    | inr b => Some b
+    | _ => None
+end.
+
+Definition mlefts {A B : Type} (x : M (A + B)) : M A :=
+  mcatOptions (fmap sum_left x).
+
+Definition mrights {A B : Type} (x : M (A + B)) : M B :=
+  mcatOptions (fmap sum_right x).
+
+Definition mpartitionSums {A B : Type} (x : M (A + B)) : M A * M B :=
+  (mlefts x, mrights x).
+
+Definition mmapOption {A B : Type} (f : A -> option B) (x : M A) : M B :=
+  mcatOptions (fmap f x).
+
+End MonadFailFuns.
+Print mfilter.
+Check mfilter _.
+Arguments mfilter : default implicits.
+Check mfilter.
+Arguments mfilter {M instM instMF A} _ _.
+Check mfilter.
+Arguments mpartition {M instM instMF A} _ _.
+Arguments mcatOptions {M instM instMF A} _.
